ArchSemTinyArm/PromisingTest.lean
@@ -1,42 +1,29 @@
-import Std.Data.HashSet
 import ArchSemTinyArm.Promising
 import ArchSemTinyArm.Basic
 
 open Sail.ArchSem
-open ArchSem.Promising
+open ArchSem.TerminatingModel
+open ArchSemTinyArm.Promising
 
 /- CR clang: there is some duplication here with sequential tests. -/
 
 def isem : SailM Unit := Out.Functions.fetch_and_execute ()
 
-def memInsert4 (addr : BitVec 64) (value : BitVec 32) (mem : InitialMem) :=
-  assert! (addr.getLsb 0) == false
-  assert! (addr.getLsb 1) == false
-  if addr.getLsb 2 then /- Upper half. -/
-    let word : BitVec 64 := mem.getD (addr >>> 3) (BitVec.zero 64)
-    let word := word &&& (BitVec.ofInt 64 (0xFFFFFFFF))
-    let word := word ||| (value.zeroExtend 64 <<< 32)
-    mem.insert (addr >>> 3) word
-  else /- Lower half. -/
-    let word := mem.getD (addr >>> 3) (BitVec.zero 64)
-    let word := word &&& (BitVec.ofInt 64 (0xFFFFFFFF <<< 32))
-    let word := word ||| value
-    mem.insert (addr >>> 3) word
-
-def extractRegs (regs : List (Fin n × Register)) (mstate : ModelState n)
+def extractRegs (regs : List (Fin n × Register)) (archState : ArchState n)
     : List (Option String) :=
   let getRegValue (tid : Fin n) (reg : Register)
       : Option (Arch.register_type reg) :=
-    mstate.threadStates[tid].regs.get? reg |> Option.map Prod.fst
+    archState.regs[tid].get? reg
   regs.map (fun (tid,reg) => getRegValue tid reg |> Option.map reprStr)
 
-def prepareTestResults [BEq α] [Hashable α] (extractor : ModelState n → α)
-    (res : ExecutionMonad.NResult (ModelState n × String) (ModelState n × ModelState n) )
-    : List String × Std.HashSet α :=
-  let errs := res.errors.map (fun (_mstate,err) => err)
-  let finalStates := res.results.map Prod.snd
-  let results := finalStates.map extractor
-  (errs, Std.HashSet.ofList results)
+def prepareTestResults [BEq α] (extractor : ArchState n → α)
+    (res : ListSet (ModelResult n Unit termCond))
+    : ListSet String × ListSet α :=
+  res.toList.foldl (fun (errs,results) r => match r with
+    | .finalState s _ => (errs, extractor s :: results)
+    | .flagged () => (errs.insert "Flagged", results)
+    | .error msg => (errs.insert msg, results)
+    ) (ListSet.empty, ListSet.empty)
 
 namespace EOR
 
@@ -47,35 +34,37 @@ def initialRegs : RegisterMap :=
   |>.insert .R1 (BitVec.ofNat 64 0x11)
   |>.insert .R2 (BitVec.ofNat 64 0x101)
 
-def initialMem : InitialMem :=
-  (Std.ExtHashMap.emptyWithCapacity 32)
-  |> memInsert4 0x500 0xca020020
+def initialMem : MemoryMap :=
+  MemoryMap.empty
+  |>.insert 4 0x500 0xca020020
 
 abbrev nThreads := 1
-def initialState : ModelState nThreads := {
-  threadStates := ⟨#[
-    ThreadState.init initialRegs
+def initialState : ArchState nThreads := {
+  regs := ⟨#[
+    initialRegs
   ], rfl⟩,
-  initmem := initialMem,
-  mem := []
+  memory := initialMem,
+  addressSpace := ()
 }
 
 def terminationCondition : TerminationCondition nThreads := fun _tid regs =>
   regs.get? ._PC == .some (BitVec.ofNat 64 0x504)
 
 def fuel := 1
-def finalStateExtractor : ModelState nThreads → List (Option String)
+def finalStateExtractor : ArchState nThreads → List (Option String)
   := extractRegs [(0, .R0)]
-def expectedFinalStates := Std.HashSet.ofList [[some "0x0000000000000110#64"]]
+def expectedResults := ListSet.ofList [[some "0x0000000000000110#64"]]
 
-def results := run fuel isem terminationCondition initialState
-def output := prepareTestResults finalStateExtractor results
+def naiveModel : ComputationalTerminatingModel Unit := createNaiveModel sailTinyArmIsem fuel
+def promiseFirstModel : ComputationalTerminatingModel Unit := createPromiseFirstModel sailTinyArmIsem fuel
 
-def promiseFirstResults := runPromiseFirst fuel isem terminationCondition initialState
-def promiseFirstOutput := prepareTestResults finalStateExtractor results
+def naiveOutput := naiveModel terminationCondition initialState
+def naiveResults := prepareTestResults finalStateExtractor naiveOutput
+def promiseFirstOutput := promiseFirstModel terminationCondition initialState
+def promiseFirstResults := prepareTestResults finalStateExtractor promiseFirstOutput
 
-#guard output == promiseFirstOutput
-#guard output == ([], expectedFinalStates)
+#guard naiveResults == promiseFirstResults
+#guard naiveResults == ([], expectedResults)
 
 end EOR
 
@@ -110,26 +99,26 @@ def initialRegsT1 : RegisterMap :=
   |>.insert .R4 (BitVec.ofNat 64 0x200)
   |>.insert .R5 (BitVec.ofNat 64 0x0)
 
-def initialMem : InitialMem :=
-  (Std.ExtHashMap.emptyWithCapacity 32)
+def initialMem : MemoryMap :=
+  MemoryMap.empty
   /- Thread 0 @ 0x500 -/
-  |> memInsert4 0x500 0xf8206822  /- STR X2, [X1, X0] -/
-  |> memInsert4 0x504 0xf8236885  /- STR X5, [X4, X3] -/
+  |>.insert 4 0x500 0xf8206822  /- STR X2, [X1, X0] -/
+  |>.insert 4 0x504 0xf8236885  /- STR X5, [X4, X3] -/
   /- Thread 1 @ 0x600 -/
-  |> memInsert4 0x600 0xf8636885  /- LDR X5, [X4, X3] -/
-  |> memInsert4 0x604 0xf8606822  /- LDR X2, [X1, X0] -/
+  |>.insert 4 0x600 0xf8636885  /- LDR X5, [X4, X3] -/
+  |>.insert 4 0x604 0xf8606822  /- LDR X2, [X1, X0] -/
   /- Backing memory so the addresses exist -/
-  |>.insert (0x1100 >>> 3) 0x0
-  |>.insert (0x1200 >>> 3) 0x0
+  |>.insert 8 0x1100 0x0
+  |>.insert 8 0x1200 0x0
 
 abbrev nThreads := 2
-def initialState : ModelState nThreads := {
-  threadStates := ⟨#[
-    ThreadState.init initialRegsT0,
-    ThreadState.init initialRegsT1
+def initialState : ArchState nThreads := {
+  regs := ⟨#[
+    initialRegsT0,
+    initialRegsT1
   ], rfl⟩,
-  initmem := initialMem,
-  mem := []
+  memory := initialMem,
+  addressSpace := ()
 }
 
 def terminationCondition : TerminationCondition nThreads := fun tid regs =>
@@ -138,21 +127,23 @@ def terminationCondition : TerminationCondition nThreads := fun tid regs =>
   | 1 => regs.get? ._PC == .some (BitVec.ofNat 64 0x608)
 
 def fuel := 6
-def finalStateExtractor : ModelState nThreads → List (Option String)
+def finalStateExtractor : ArchState nThreads → List (Option String)
   := extractRegs [(1, .R5), (1, .R2)]
-def expectedFinalStates := Std.HashSet.ofList [
+def expectedResults := ListSet.ofList [
   [some "0x0000000000000001#64", some "0x000000000000002a#64"],
   [some "0x0000000000000001#64", some "0x0000000000000000#64"],
   [some "0x0000000000000000#64", some "0x000000000000002a#64"],
   [some "0x0000000000000000#64", some "0x0000000000000000#64"]]
 
-def results := run fuel isem terminationCondition initialState
-def output := prepareTestResults finalStateExtractor results
+def naiveModel : ComputationalTerminatingModel Unit := createNaiveModel sailTinyArmIsem fuel
+def promiseFirstModel : ComputationalTerminatingModel Unit := createPromiseFirstModel sailTinyArmIsem fuel
 
-def promiseFirstResults := runPromiseFirst fuel isem terminationCondition initialState
-def promiseFirstOutput := prepareTestResults finalStateExtractor results
+def naiveOutput := naiveModel terminationCondition initialState
+def naiveResults := prepareTestResults finalStateExtractor naiveOutput
+def promiseFirstOutput := promiseFirstModel terminationCondition initialState
+def promiseFirstResults := prepareTestResults finalStateExtractor promiseFirstOutput
 
-#guard output == promiseFirstOutput
-#guard output == ([], expectedFinalStates)
+#guard naiveResults == promiseFirstResults
+#guard naiveResults == ([], expectedResults)
 
 end MP
