ArchsemLean/TerminatingModel.lean
@@ -1,0 +1,62 @@
+import Std.Data.ExtHashMap
+import Std.Data.HashSet
+import ArchsemLean.Common
+import Sail
+
+open Sail.ArchSem
+
+-- CR clang: comment this code similar to archsem comments.
+
+namespace ArchSem.TerminatingModel
+
+variable [ArchExtra]
+abbrev Address := BitVec Arch.addr_size
+def MemoryMap := Std.HashMap Address (BitVec 8)
+deriving BEq
+def MemoryMap.empty : MemoryMap := Std.HashMap.emptyWithCapacity 1024
+def MemoryMap.insertByte (addr : Address) (byte : BitVec 8) (mem : MemoryMap)
+    : MemoryMap :=
+  mem.insert addr byte
+def MemoryMap.insert (size : Nat) (addr : Address) (word : BitVec (8 * size)) (mem : MemoryMap)
+    : MemoryMap :=
+  let bytes := Sail.bitvec_to_vecbytes word
+  (List.finRange size).foldl (fun m i => m.insertByte (addr + i.val) bytes[i]) mem
+
+-- CR clang: MemoryMap manipulation functions
+-- CR clang: RegisterMap should probably be just a DHasmMap.
+def RegisterMap [ArchExtra] := Std.DHashMap Arch.register Arch.register_type
+deriving BEq
+def RegisterMap.empty [ArchExtra] : RegisterMap := Std.DHashMap.emptyWithCapacity 64
+-- CR clang: RegisterMap manipulation functions
+abbrev TerminationCondition [ArchExtra] (nThreads : Nat) := Fin nThreads → RegisterMap → Bool
+
+structure ArchState (nThreads : Nat) where
+  memory : MemoryMap
+  addressSpace : Arch.addr_space
+  regs : Vector RegisterMap nThreads
+deriving BEq
+
+def ArchState.has_terminated (termCond : TerminationCondition nThreads)
+    (s : ArchState nThreads) : Prop :=
+  ∀ tid : Fin nThreads, termCond tid s.regs[tid]
+
+-- def HasTerminated ...
+-- (List.finRange nThreads).all (fun tid => termCond tid s.regs[tid])
+
+inductive ModelResult (nThreads : Nat) (Flag : Type) (termCond : TerminationCondition nThreads)
+  | finalState (s : ArchState nThreads) (t : s.has_terminated termCond)
+  | flagged (f : Flag)
+  | error (msg : String)
+
+instance [BEq Flag] : BEq (ModelResult n Flag termCond) where
+  beq
+    | .finalState s₁ _, .finalState s₂ _ => s₁ == s₂
+    | .flagged f₁, .flagged f₂ => f₁ == f₂
+    | .error m₁, .error m₂ => m₁ == m₂
+    | _, _ => false
+
+def ComputationalTerminatingModel (Flag : Type) [DecidableEq Flag] :=
+  {nThreads : Nat} → (termCond : TerminationCondition nThreads) →
+  ArchState nThreads → ListSet (ModelResult nThreads Flag termCond)
+
+end ArchSem.TerminatingModel
